Brought TODO list up to speed + skeleton for SemanticsSafetyLike

CommonST.v
@@ -105,17 +105,17 @@ Definition hrsat2 {K : level} (P1 P2 : @prg K) (r : rel_hprop) : Prop :=
 
 (**************************************************************************)
 
-Definition input_totality {K : level} : Prop :=
+Definition input_totality (K : level) : Prop :=
   forall (P : prg K) m e1 e2,
     is_input e1  -> is_input e2 -> fstopped m = false ->
     psem P (fsnoc m e1) -> psem P (fsnoc m e2). 
 
 
-Definition determinacy {K : level} : Prop :=
+Definition determinacy (K : level) : Prop :=
   forall (P : prg K) t1 t2,
     sem K P t1 -> sem K P t2 -> traces_match t1 t2.
 
-Definition semantic_safety_like {K : level} : Prop :=
+Definition semantics_safety_like (K : level) : Prop :=
   forall t P,
     ~ sem K P t -> inf t ->
     (exists m ebad, psem P m /\ prefix (fsnoc m ebad) t /\ ~ psem P (fsnoc m ebad)).
