SemanticsSafetyLike.v
@@ -1,0 +1,32 @@
+Require Import Events.
+Require Import TraceModel.
+Require Import Properties.
+Require Import CommonST.
+
+Section Main.
+
+Variable prg  : Set.
+Variable ctx  : Set.
+Variable plug : prg -> ctx -> prg.
+
+Variable cfg : Set.
+Variable init : prg -> cfg.
+Variable step : cfg -> event -> cfg -> Prop.
+
+Definition stuck (c:cfg) : Prop :=  forall e c', ~step c e c'.
+
+CoInductive sem' : cfg -> trace -> Prop :=
+| SStop : forall c, stuck c -> sem' c tstop
+| SCons : forall c e c' t, step c e c' -> sem' c' t -> sem' c (tcons e t).
+
+Definition sem (p:prg) : trace -> Prop := sem' (init p).
+
+Lemma non_empty_sem : forall P, exists t, sem P t.
+Admitted.
+
+Definition lang : level := @Build_level prg ctx plug sem non_empty_sem.
+
+Lemma tgt_sem : semantics_safety_like lang.
+Admitted.
+
+End Main.
